\documentclass{article}
\usepackage{blindtext}
\usepackage[utf8]{inputenc}
\usepackage{amsmath}

\title{Homework one}
\author{U201514545 Bachelar Hu}
\date{\today}

\begin{document}
\maketitle
\section{}
Porve is a cycle.\newline
Assuming $Mv = {\lambda}v$

\begin{itemize}
    \item
        $1 \implies 3$\newline
        $\forall{x} \quad x^{T}Mx\geq0  \implies\forall{x} \quad x^{T}{\lambda}vx \geq 0
        \implies\forall{x} \quad {\lambda}x^{T}vx \geq a$\newline
        so all eigenvalue of M is non-negtive
    \item
        $2 \implies 1$\newline
        $M=BB^{T}\implies x^{T}Mx=x^{T}BB^{T}x \implies x^{T}Mx=(B^{T}x)^{T}B^{T}x\geq0$
    \item
        $3 \implies 2$\newline
        The matrix $M$ is symmetric matrix.so there exists an on
        orthogonal matrix $Q$ such that $Q^{T}MQ=D$, where $D$ is the
        diagonal matrix

        \[D=\begin{bmatrix}
            \lambda_1 & 0 & 0 & 0 \\
            0 & \lambda_2 & 0 & 0 \\
            \vdots & \cdots & \ddots & \vdots \\
            0 & 0 & \cdots & \lambda_n
        \end{bmatrix}\]

        \[
            M = {Q^{-1}}^{T}
            \begin{bmatrix}
            \lambda_1 & 0 & 0 & 0 \\
            0 & \lambda_2 & 0 & 0 \\
            \vdots & \cdots & \ddots & \vdots \\
            0 & 0 & \cdots & \lambda_n
            \end{bmatrix}
            Q^{-1}
        \]

        \[
            M = {Q^{-1}}^{T}
            \begin{bmatrix}
                \sqrt{\lambda_1} & 0 & 0 & 0 \\
                0 & \sqrt{\lambda_2} & 0 & 0 \\
                \vdots & \cdots & \ddots & \vdots \\
                0 & 0 & \cdots & \sqrt{\lambda_n}
            \end{bmatrix}
            \begin{bmatrix}
                \sqrt{\lambda_1} & 0 & 0 & 0 \\
                0 & \sqrt{\lambda_2} & 0 & 0 \\
                \vdots & \cdots & \ddots & \vdots \\
                0 & 0 & \cdots & \sqrt{\lambda_n}
            \end{bmatrix}
            Q^{-1}
        \]
        Let
        \[
            B = {Q^{-1}}^{T}
            \begin{bmatrix}
                \sqrt{\lambda_1} & 0 & 0 & 0 \\
                0 & \sqrt{\lambda_2} & 0 & 0 \\
                \vdots & \cdots & \ddots & \vdots \\
                0 & 0 & \cdots & \sqrt{\lambda_n}
            \end{bmatrix}
        \]

        So
        \[
            M=BB^{T}
        \]


\end{itemize}

\section{}
For a sample of vectors $x_i=(x_{i1},\dots,x_{ik})^\top$, with $i=1,\dots,n$, the sample mean vector is
\[ \bar{x}=\frac{1}{n} \sum_{i=1}^n x_i \, , \]
and the sample covariance matrix is
\[ Q = \frac{1}{n} \sum_{i=1}^n (x_i-\bar{x})(x_i-\bar{x})^\top \, .  \]
For a nonzero vector $y$, we have
\[ y^\top Qy = y^\top\left(\frac{1}{n} \sum_{i=1}^n (x_i-\bar{x})(x_i-\bar{x})^\top\right) y \]
\[ = \frac{1}{n} \sum_{i=1}^n y^\top (x_i-\bar{x})(x_i-\bar{x})^\top y \]
\[ = \frac{1}{n} \sum_{i=1}^n ((x_i-\bar{x})^\top y)^\top ((x_i-\bar{x})^\top y) \]
\[ = \frac{1}{n} \sum_{i=1}^n \left( (x_i-\bar{x})^\top y \right)^2 \geq 0 \, . \quad (*) \]
Therefore, $Q$ is always positive semi-definite

\section{}
\subsection{}
\begin{itemize}
    \item
        $Cu_i = (A + B)u_i = Au_i + Bu_i = {\alpha}_iu_i + {\beta}_iu_i =
        ({\alpha}_i + {\beta}_i )u_i$
    \item
        $Du_i = (A - B)u_i = Au_i - Bu_i = {\alpha}_iu_i - {\beta}_iu_i =
        ({\alpha}_i - {\beta}_i )u_i$
    \item
        matrix multiplication is associative\newline
        $Eu_i = (AB)u_i = A(Bu_i) = {\beta}_iAu_i = {\alpha}_i{\beta}_iu_i$
    \item
        $A\mathbf{v} = \lambda\mathbf{v} \implies A^{-1}A\mathbf{v} = \lambda
    A^{-1}\mathbf{v} \implies A^{-1}\mathbf{v} = \frac{1}{\lambda}\mathbf{v}$
    $Fu_i=A^{-1}B={\alpha}_i^{-1}\beta_iu_i$
\end{itemize}
\subsection{}
    \[
        F=
        \begin{bmatrix}
            \mathbf{A} & 0 \\
            0 & \mathbf{B}
        \end{bmatrix}
    \]

    \[
        M=\begin{bmatrix}
            \mathbf{u_i}\\
            0
        \end{bmatrix}
    \]

    ${\lambda}_i$ and
    $
    \begin{bmatrix}
        \mathbf{u_i}\\
        0
    \end{bmatrix}
    $
    is one answer, here is the prove
    \[
        FM=
        \begin{bmatrix}
            \mathbf{A} & 0 \\
            0 & \mathbf{B}
        \end{bmatrix}
        \begin{bmatrix}
            \mathbf{u_i}\\
            0
        \end{bmatrix}
        =
        \begin{bmatrix}
            A\mathbf{u_i}\\
            0
        \end{bmatrix}
        =
        \lambda_i
        \begin{bmatrix}
            \mathbf{u_i}\\
            0
        \end{bmatrix}
        =
        {\lambda_i}
        M
    \]

    Similarly, ${\beta}_i$ and $ \begin{bmatrix}  0 \\ \mathbf{u_i} \end{bmatrix}$ is one
    answer

\end{document}

